[Progress] Incorporate weakest preconditions to language structure and adapt simulations to language constructs.

src/Framework/Layer/HoareLogic.v
@@ -1,5 +1,5 @@
 Require Export String Datatypes.
-Require Import Primitives SeparationLogic Layer.Language.
+Require Import Primitives SeparationLogic Layer.Operation Layer.Language.
 
 Set Implicit Arguments.
 
@@ -7,79 +7,71 @@ Create HintDb specs.
 
 Instance addr_eq_dec: EqDec addr := addr_dec.
 
-Module HoareLogic (Ops: Operation).
-  Module Lang := Language Ops.
-  Import Ops Lang.
-  Export Lang.
+Section HoareLogic.
+  Variable Ops: Operation.
+  Variable Lang: Language Ops.
+  
+  Definition Marker {T} (s: string) (p: Lang.(prog) T) := True.
 
-Definition Marker {T} (s: string) (p: prog T) := True.
-
-(** ** Hoare logic *)
-Definition pre_condition := state -> Prop.
-Definition post_condition {T: Type} := T -> state -> Prop.
-Definition crash_condition := state -> Prop.
-Definition oracle_pre_condition {T: Type} := oracle -> prog T -> state -> Prop.
-Definition oracle_post_condition {T: Type} := oracle -> state -> T -> state -> Prop.
-Definition oracle_crash_condition := oracle -> state -> state -> Prop.
-
-Definition hoare_triple {T: Type}
-           (opre: @oracle_pre_condition T)
-           (pre: pre_condition)
-           (p: prog T)
-           (post: @post_condition T)
-           (crash: crash_condition)
-           (opost: oracle_post_condition)
-           (ocrash: oracle_crash_condition):=
+  Definition pre_condition' := Lang.(state) -> Prop.
+  Definition post_condition' {T: Type} := T -> Lang.(state) -> Prop.
+  Definition crash_condition' := Lang.(state) -> Prop.
+  
+  Definition oracle_pre_condition' {T: Type} := Lang.(oracle) -> Lang.(prog) T -> Lang.(state) -> Prop.
+  Definition oracle_post_condition' {T: Type} := Lang.(oracle) -> Lang.(state) -> T -> Lang.(state) -> Prop.
+  Definition oracle_crash_condition' := Lang.(oracle) -> Lang.(state) -> Lang.(state) -> Prop.
+  
+Definition hoare_triple' {T: Type}
+           (opre: @oracle_pre_condition' T)
+           (pre: pre_condition')
+           (p: Lang.(prog) T)
+           (post: @post_condition' T)
+           (crash: crash_condition')
+           (opost: oracle_post_condition')
+           (ocrash: oracle_crash_condition'):=
   fun o s =>
     opre o p s ->
     pre s ->
     (exists ret,
-        exec o s p ret /\
+        Lang.(exec) o s p ret /\
         ((exists s' r,
              ret = Finished s' r
              /\ post r s' /\ opost o s r s') \/
          (exists s',
              ret = Crashed s' /\ crash s' /\ ocrash o s s')))%type.
 
-Notation
-  "<< o , s >> 'PRE:' pre 'PROG:' p << r , s' >> 'POST:' post 'CRASH:' crash 'OPRE:' opre 'OPOST:' opost 'OCRASH:' ocrash" :=
-  (hoare_triple
-          (fun o p' s => oracle_ok p' o s /\ opre)
-          (fun s => pre)
-          p
-          (fun r s' => post)
-          (fun s' => crash)
-          (fun o s r s' => opost)
-          (fun o s s' => ocrash)
-          o s)      
-    (at level 10, o at next level, s at next level, s' at next level, opre at next level, pre at next level, p at next level, r at next level, post at next level, crash at next level, opost at next level, ocrash at next level,
-     format "'[v' '[  ' '<<' o ','  s '>>' '//' '[' 'PRE:' '//' pre ']' '//' '[' 'PROG:' '//' p ']' ']' '//' '[  ' '<<' r ','  s' '>>' '//' '[' 'POST:' '//' post ']' '//' '[' 'CRASH:' '//' crash ']' '//' '[' 'OPRE:' '//' opre ']' '//' '[' 'OPOST:' '//' opost ']' '//' '[' 'OCRASH:' '//' ocrash ']' ']' ']'").
+Arguments post_condition' : clear implicits.
+Arguments oracle_pre_condition' : clear implicits.
+Arguments oracle_post_condition' : clear implicits.
+Arguments hoare_triple' : clear implicits.
 
-Notation
-  "<< o , s >> 'PRE:' pre 'PROG:' p << r , s' >> 'POST:' post 'CRASH:' crash" :=
-  (hoare_triple
-          (fun o p' s => oracle_ok p' o s)
-          (fun s => pre)
-          p
-          (fun r s' => post)%pred
-          (fun s' => crash)%pred
-          (fun o s r s' => True)
-          (fun o s s' => True)
-          o s)      
-    (at level 10, o at next level, s at next level, s' at next level, pre at next level, p at next level, r at next level, post at next level, crash at next level,
-     format "'[v' '[  ' '<<' o ','  s '>>' '//' '[' 'PRE:' '//' pre ']' '//' '[' 'PROG:' '//' p ']' ']' '//' '[  ' '<<' r ','  s' '>>' '//' '[' 'POST:' '//' post ']' '//' '[' 'CRASH:' '//' crash ']' ']' ']'").
+Record HoareLogic :=
+  {
+    pre_condition := pre_condition';
+    post_condition := post_condition';
+    crash_condition := crash_condition';
+
+    oracle_pre_condition := oracle_pre_condition';
+    oracle_post_condition := oracle_post_condition';
+    oracle_crash_condition := oracle_crash_condition';
+
+    hoare_triple := hoare_triple';
+  }.
+
+End HoareLogic.
+
 
 Theorem crash_impl:
-  forall T (p: prog T) opre pre post (crash1 crash2: crash_condition) opost ocrash o s,
-    hoare_triple opre pre p post crash1 opost ocrash o s -> 
+  forall O (Lang: Language O) HL T (p: Lang.(prog) T) opre pre post (crash1 crash2: crash_condition HL) opost ocrash o s,
+    hoare_triple HL opre pre p post crash1 opost ocrash o s -> 
     (forall s',
       Marker "crash_impl implication for" p ->
       pre s ->
       crash1 s' ->
       crash2 s') ->
-    hoare_triple opre pre p post crash2 opost ocrash o s.
+    hoare_triple HL opre pre p post crash2 opost ocrash o s.
 Proof.
-  unfold Marker, hoare_triple; intros.
+  unfold Marker, hoare_triple, hoare_triple' ; intros.
   edestruct H; eauto.
   cleanup.
   split_ors; cleanup;
@@ -88,16 +80,16 @@ Qed.
 
 
 Theorem post_impl:
-  forall T (p: prog T) opre pre (post1 post2: post_condition) crash opost ocrash o s,
-    hoare_triple opre pre p post1 crash opost ocrash o s -> 
+  forall O (Lang: Language O) HL T (p: Lang.(prog) T) opre pre (post1 post2: post_condition HL T) crash opost ocrash o s,
+    hoare_triple HL opre pre p post1 crash opost ocrash o s -> 
     (forall r s',
       Marker "post_impl implication for" p ->
       pre s ->
       post1 r s' ->
       post2 r s') ->
-    hoare_triple opre pre p post2 crash opost ocrash o s.
+    hoare_triple HL opre pre p post2 crash opost ocrash o s.
 Proof.
-  unfold Marker, hoare_triple; intros.
+  unfold Marker, hoare_triple, hoare_triple'; intros.
   edestruct H; eauto.
   cleanup.
   split_ors; cleanup;
@@ -106,37 +98,37 @@ Proof.
 Qed.
 
 Theorem pre_impl:
-  forall T (p: prog T) opre (pre1 pre2: pre_condition) post crash opost ocrash o s,
-    hoare_triple opre pre1 p post crash opost ocrash o s -> 
+  forall O (Lang: Language O) HL T (p: Lang.(prog) T) opre (pre1 pre2: pre_condition HL) post crash opost ocrash o s,
+    hoare_triple HL opre pre1 p post crash opost ocrash o s -> 
     ( Marker "pre_impl implication for" p ->
       pre2 s ->
       pre1 s ) ->
-    hoare_triple opre pre2 p post crash opost ocrash o s.
+    hoare_triple HL opre pre2 p post crash opost ocrash o s.
 Proof.
-  unfold Marker, hoare_triple; intros.
+  unfold Marker, hoare_triple, hoare_triple'; intros.
   edestruct H; eauto.
 Qed.
 
 Theorem remove_oracle_conditions:
-  forall T (p: prog T) (opre: oracle_pre_condition) pre post crash (opost: oracle_post_condition) (ocrash: oracle_crash_condition) o s,
-  hoare_triple opre pre p post crash (fun _ _ _ _ => True) (fun _ _ _ => True) o s -> 
+  forall O (Lang: Language O) HL T (p: Lang.(prog) T) (opre: oracle_pre_condition HL T) pre post crash (opost: oracle_post_condition HL T) (ocrash: oracle_crash_condition HL) o s,
+  hoare_triple HL opre pre p post crash (fun _ _ _ _ => True) (fun _ _ _ => True) o s -> 
   (forall r s',
      Marker "opost for" p ->
      opre o p s ->
      pre s ->
-     exec o s p (Finished s' r) ->
+     Lang.(exec) o s p (Finished s' r) ->
      post r s' ->
      opost o s r s') ->
   (forall s',
       Marker "ocrash for" p ->
       opre o p s ->
       pre s ->
-      exec o s p (Crashed s') ->
+      Lang.(exec) o s p (Crashed s') ->
       crash s' ->
       ocrash o s s') ->
-   hoare_triple opre pre p post crash opost ocrash o s.
+   hoare_triple HL opre pre p post crash opost ocrash o s.
 Proof.
-  unfold Marker, hoare_triple; intros.
+  unfold Marker, hoare_triple, hoare_triple'; intros.
   edestruct H; eauto; cleanup.
   
   split_ors; cleanup;
@@ -145,38 +137,38 @@ Proof.
 Qed.
 
 Theorem pre_impl_false:
-  forall T (p: prog T) opre (pre: pre_condition) post crash opost ocrash o s,
+  forall O (Lang: Language O) HL T (p: Lang.(prog) T) opre (pre: pre_condition HL) post crash opost ocrash o s,
     ( Marker "pre_impl_false implication for" p ->
       pre s ->
       False ) ->
-    hoare_triple opre pre p post crash opost ocrash o s.
+    hoare_triple HL opre pre p post crash opost ocrash o s.
 Proof.
-  unfold Marker, hoare_triple; intros.
+  unfold Marker, hoare_triple, hoare_triple'; intros.
   edestruct H; eauto.
 Qed.
 
 
 (*
-Theorem hoare_triple_equivalence :
-  forall T (p p': prog T) o s pre post crash ap ac,
-    hoare_triple pre p post crash ap ac o s ->
-    prog_equiv p p' ->
-    hoare_triple pre p' post crash ap ac o s.
+Theorem hoare_triple'_equivalence :
+  forall T (p p': Lang.(prog) T) o s pre post crash ap ac,
+    hoare_triple' pre p post crash ap ac o s ->
+    Lang.(prog)_equiv p p' ->
+    hoare_triple' pre p' post crash ap ac o s.
 Proof.
-  unfold hoare_triple; intros.
+  unfold hoare_triple'; intros.
   edestruct H; eauto; cleanup.
   match goal with
   | [ H: _ ~= _ |- _ ] =>
     edestruct H; eauto
   end.
-  unfold exec in *.
+  unfold Lang.(exec) in *.
   eauto.
 Qed.
 
 Ltac monad_simpl_one :=
   match goal with
-  | [ |- hoare_triple _ (Bind (Bind _ _) _) _ _ _ _ _ _ _] =>
-    eapply hoare_triple_equivalence;
+  | [ |- hoare_triple' _ (Bind (Bind _ _) _) _ _ _ _ _ _ _] =>
+    eapply hoare_triple'_equivalence;
     [ | apply bind_assoc ]
   end.
 
@@ -184,39 +176,37 @@ Ltac monad_simpl := repeat monad_simpl_one.
 *)
 
 Theorem ret_ok:
-  forall P o s T (v: T),
-    << o, s >>
-    PRE:
-     (P s)
-    PROG:
-     (Ret v)
-    << r, s' >>
-    POST:
-     (P s' /\ r = v /\ s' = s)
-    CRASH:
-     (P s' /\ s' = s).
+  forall O (L: Language O) (HL: HoareLogic L) P o s T (v: T),
+    (hoare_triple HL
+          (fun o p' s => o = [Cont O] \/ o = [Crash O])
+          (fun s => P s)
+          (Ret v)
+          (fun r s' => P s' /\ r = v /\ s' = s)%pred
+          (fun s' => P s' /\ s' = s)%pred
+          (fun o s r s' => True)
+          (fun o s s' => True)
+          o s).
 Proof.
   intros.
-  unfold hoare_triple; intros.
-  destruct_lift H; subst.
+  unfold hoare_triple, hoare_triple'; intros.
   split_ors; eexists;
   intuition (try econstructor; eauto).
   do 2 eexists; eauto.
 Qed.
 
 Theorem bind_ok:
-  forall T T' (p1: prog T) (p2: T -> prog T') (opre opre1 opre2: oracle_pre_condition) (pre1 pre2: pre_condition) post1 post2 (crash1 crash2: crash_condition) (opost opost1 opost2: oracle_post_condition) (ocrash ocrash1 ocrash2 : oracle_crash_condition) o s, 
+  forall O (Lang: Language O) (HL: HoareLogic Lang) T T' (p1: Lang.(prog) T) (p2: T -> Lang.(prog) T') (opre opre1 opre2: oracle_pre_condition HL _) (pre1 pre2: pre_condition HL) post1 post2 (crash1 crash2: crash_condition HL) (opost opost1 opost2: oracle_post_condition HL _) (ocrash ocrash1 ocrash2 : oracle_crash_condition HL) o s, 
   (forall o1,
       Marker "bind_ok spec for" p1 ->
       (exists o2, o = o1++o2) ->
-      hoare_triple opre1 pre1 p1 post1 crash1 opost1 ocrash1 o1 s) ->
+      hoare_triple HL opre1 pre1 p1 post1 crash1 opost1 ocrash1 o1 s) ->
   (forall r s',
-     Marker "bind_ok post1 -> pre2 for" (Bind p1 p2) ->
+     @Marker _ Lang _ "bind_ok post1 -> pre2 for" (Bind p1 p2) ->
      pre1 s ->
      post1 r s' ->
      pre2 s') ->
   (forall s',
-     Marker "bind_ok crash1 -> crash2 for" (Bind p1 p2) ->
+     @Marker _ Lang _  "bind_ok crash1 -> crash2 for" (Bind p1 p2) ->
      pre1 s ->
      crash1 s' -> crash2 s') ->
   (forall o1 o2 r s',
@@ -225,39 +215,39 @@ Theorem bind_ok:
       pre1 s ->
       post1 r s'->
       o = o1 ++ o2 ->
-      exec o1 s p1 (Finished s' r) ->
-      hoare_triple opre2 pre2 (p2 r) post2 crash2 opost2 ocrash2 o2 s') ->
-  (Marker "bind_ok opre -> opre1 /\ opre2 for" (Bind p1 p2) ->
+      Lang.(exec) o1 s p1 (Finished s' r) ->
+      hoare_triple HL opre2 pre2 (p2 r) post2 crash2 opost2 ocrash2 o2 s') ->
+  (@Marker _ Lang _  "bind_ok opre -> opre1 /\ opre2 for" (Bind p1 p2) ->
       opre o (Bind p1 p2) s ->
       exists o1 o2,
       o = o1++o2 /\
       opre1 o1 p1 s /\
       (forall s' r,
-          exec o1 s p1 (Finished s' r) ->
+          Lang.(exec) o1 s p1 (Finished s' r) ->
           opre2 o2 (p2 r) s')) ->
   (forall o1 o2 s1 s2 r1 r2,
-      Marker "bind_ok opost1 /\ opost2 -> opost for" (Bind p1 p2) ->
+      @Marker _ Lang _  "bind_ok opost1 /\ opost2 -> opost for" (Bind p1 p2) ->
       o = o1++o2 ->
       opre1 o1 p1 s ->
       opost1 o1 s r1 s1 ->
       opost2 o2 s1 r2 s2 ->
       opost o s r2 s2) ->
   (forall o1 o2 s1 s2 r1,
-      Marker "bind_ok opost1 /\ ocrash2 -> ocrash for" (Bind p1 p2) ->
+      @Marker _ Lang _  "bind_ok opost1 /\ ocrash2 -> ocrash for" (Bind p1 p2) ->
       o = o1++o2 ->
       opre1 o1 p1 s ->
       opost1 o1 s r1 s1 ->
       ocrash2 o2 s1 s2 ->
       ocrash o s s2) ->
   (forall o1 o2 s1,
-      Marker "bind_ok ocrash1 -> ocrash for" (Bind p1 p2) ->
+      @Marker _ Lang _  "bind_ok ocrash1 -> ocrash for" (Bind p1 p2) ->
       o = o1++o2 ->
       opre1 o1 p1 s ->
       ocrash1 o1 s s1 ->
       ocrash o s s1) ->
-  hoare_triple opre pre1 (Bind p1 p2) post2 crash2 opost ocrash o s.
+  hoare_triple HL opre pre1 (Bind p1 p2) post2 crash2 opost ocrash o s.
 Proof.
-  unfold Marker, hoare_triple; intros.
+  unfold Marker, hoare_triple, hoare_triple'; intros.
   simpl in *; cleanup.
   edestruct H3; eauto; cleanup.
   (* rewrite H0 in H6. *)
@@ -268,8 +258,10 @@ Proof.
   - edestruct H2; eauto.
     cleanup.
     split_ors; cleanup;
-      eexists; split; eauto.
+    eexists; split; eauto.
+    econstructor; eauto.
     left; do 2 eexists; repeat split; eauto.
+    econstructor; eauto.
     right; eexists; repeat split; eauto.
     
   - 
@@ -279,10 +271,9 @@ Proof.
     right; eexists; intuition eauto.
 Qed.
 
-Global Opaque Marker.
 
-Hint Extern 1 (hoare_triple _ _ (Ret _) _ _ _ _ _ _) => eapply ret_ok : specs.
-Hint Extern 1 (hoare_triple _ _ (Bind _ _) _ _ _ _ _ _) => eapply bind_ok : specs.
+Hint Extern 1 (hoare_triple _ _ _ (Ret _) _ _ _ _ _ _) => eapply ret_ok : specs.
+Hint Extern 1 (hoare_triple _ _ _ (Bind _ _) _ _ _ _ _ _) => eapply bind_ok : specs.
 
 Local Ltac ret_step :=
   eapply post_impl;
@@ -297,7 +288,7 @@ Local Ltac bind_step :=
     eapply pre_impl;
     eauto with specs
   | | |
-  | instantiate (1:= fun o p s => oracle_ok p o s); simpl; intros; eauto
+  | instantiate (1:= fun o p s => True); simpl; intros; eauto
   | instantiate (1:= fun _ _ _ _ => True); simpl; intros; eauto
   | instantiate (1:= fun _ _ _ => True); simpl; intros; eauto
   | try solve [simpl ; intros; eauto] ].
@@ -305,19 +296,62 @@ Local Ltac bind_step :=
 Ltac step :=
   intros;
   match goal with
-  | [ |- hoare_triple _ _ ?p _ _ _ _ _ _ ] => 
+  | [ |- hoare_triple _ _ _ ?p _ _ _ _ _ _ ] => 
     simpl p
   end;
   match goal with
-  | [ |- hoare_triple _ _ (Ret _) _ _ _ _ _ _ ] => 
+  | [ |- hoare_triple _ _ _ (Ret _) _ _ _ _ _ _ ] => 
     ret_step
-  | [ |- hoare_triple _ _ (Bind _ _) _ _ (fun _ _ _ _ => True) (fun _ _ _ => True) _ _ ] => 
+  | [ |- hoare_triple _ _ _ (Bind _ _) _ _ (fun _ _ _ _ => True) (fun _ _ _ => True) _ _ ] => 
     bind_step
-  | [ |- hoare_triple _ _ (Bind _ _) _ _ _ _ _ _ ] => 
-    eapply remove_oracle_conditions;
+  | [ |- hoare_triple _ _ _ (Bind _ _) _ _ _ _ _ _ ] => 
+    eapply (remove_oracle_conditions _);
     [intros; bind_step
     | try solve [ simpl; intros; eauto ]
     | try solve [ simpl; intros; eauto ] ]
   end.
 
-End HoareLogic.
+
+Notation
+  "'LOGIC:' HL << o , s >> 'OPRE:' opre 'PRE:' pre 'PROG:' p << r , s' >> 'POST:' post 'CRASH:' crash" :=
+  (HoareLogic.hoare_triple HL
+          (fun o p' s => opre)
+          (fun s => pre)
+          p
+          (fun r s' => post)%pred
+          (fun s' => crash)%pred
+          (fun o s r s' => True)
+          (fun o s s' => True)
+          o s)      
+    (at level 10, HL at next level, o at next level, s at next level, s' at next level, opre at next level, pre at next level, p at next level, r at next level, post at next level, crash at next level,
+     format "'[v' '[' 'LOGIC:'  HL ']' '//' '[  ' '<<' o ','  s '>>' '//'  '[' 'OPRE:' '//' opre ']' '//' '[' 'PRE:' '//' pre ']' '//' '[' 'PROG:' '//' p ']' ']' '//' '[  ' '<<' r ','  s' '>>' '//' '[' 'POST:' '//' post ']' '//' '[' 'CRASH:' '//' crash ']' ']' ']'").
+
+Notation
+  "'LANG:' L 'LOGIC:' HL << o , s >> 'PRE:' pre 'PROG:' p << r , s' >> 'POST:' post 'CRASH:' crash" :=
+  (HoareLogic.hoare_triple HL
+          (fun o p' s => True)
+          (fun s => pre)
+          p
+          (fun r s' => post)%pred
+          (fun s' => crash)%pred
+          (fun o s r s' => True)
+          (fun o s s' => True)
+          o s)      
+    (at level 10, L at next level, HL at next level, o at next level, s at next level, s' at next level,  pre at next level, p at next level, r at next level, post at next level, crash at next level,
+     format "'[v' '[' 'LANG:'  L ']' '//' '[' 'LOGIC:'  HL ']' '//' '[  ' '<<' o ','  s '>>' '//' '[' 'PRE:' '//' pre ']' '//' '[' 'PROG:' '//' p ']' ']' '//' '[  ' '<<' r ','  s' '>>' '//' '[' 'POST:' '//' post ']' '//' '[' 'CRASH:' '//' crash ']' ']' ']'").
+
+Notation
+  "'LANG:' L 'LOGIC:' HL << o , s >> 'PRE:' pre 'PROG:' p << r , s' >> 'POST:' post 'CRASH:' crash 'OPRE:' opre 'OPOST:' opost 'OCRASH:' ocrash" :=
+  (HoareLogic.hoare_triple HL
+          (fun o p' s => opre)
+          (fun s => pre)
+          p
+          (fun r s' => post)
+          (fun s' => crash)
+          (fun o s r s' => opost)
+          (fun o s s' => ocrash)
+          o s)      
+    (at level 10,  L at next level, HL at next level, o at next level, s at next level, s' at next level, opre at next level, pre at next level, p at next level, r at next level, post at next level, crash at next level, opost at next level, ocrash at next level,
+     format "'[v' '[' 'LANG:'  L ']' '//' '[' 'LOGIC:'  HL ']' '//' '[  ' '<<' o ','  s '>>' '//' '[' 'PRE:' '//' pre ']' '//' '[' 'PROG:' '//' p ']' ']' '//' '[  ' '<<' r ','  s' '>>' '//' '[' 'POST:' '//' post ']' '//' '[' 'CRASH:' '//' crash ']' '//' '[' 'OPRE:' '//' opre ']' '//' '[' 'OPOST:' '//' opost ']' '//' '[' 'OCRASH:' '//' ocrash ']' ']' ']'").
+
+Global Opaque Marker.
