src/Framework/Layer/HorizontalComposition.v
@@ -1,87 +1,162 @@
-Require Import Primitives Simulation Layer.Language.
+Require Import Primitives Layer.Operation Layer.Language.
 Import ListNotations.
 
 Set Implicit Arguments.
 
-Module HorizontalComposition (O1 O2: Operation) <: Operation.
-  Export O1 O2.
+Section HorizontalComposition.
+  Variable O1 O2 : Operation.
+  Variable L1 : Language O1.
+  Variable L2 : Language O2.
   
-  Inductive token :=
-  | Oracle1 : O1.oracle -> token
-  | Oracle2 : O2.oracle -> token.
+  Inductive token' :=
+  | Oracle1 : L1.(oracle) -> token'
+  | Oracle2 : L2.(oracle) -> token'.
 
-  Definition oracle := list token.
+  Definition oracle' := list token'.
 
-  Definition token_dec: forall (t t': token), {t = t'}+{t <> t'}.
+  Definition token_dec: forall (t t': token'), {t = t'}+{t <> t'}.
    decide equality.
-   apply O1.oracle_dec.
-   apply O2.oracle_dec.
+   apply L1.(oracle_dec).
+   apply L2.(oracle_dec).
   Defined.
 
-  Definition oracle_dec:= list_eq_dec token_dec.
-  Definition state := (O1.state * O2.state)%type.
+  Definition oracle_dec' := list_eq_dec token_dec.
+  Definition state' := (L1.(state) * L2.(state))%type.
 
   Inductive prog' : Type -> Type :=
-  | P1 : forall T, O1.prog T -> prog' T
-  | P2 : forall T, O2.prog T -> prog' T.
-  
-  Definition prog := prog'.
+  | P1 : forall T, L1.(prog) T -> prog' T
+  | P2 : forall T, L2.(prog) T -> prog' T.
 
-  Inductive exec': forall T, oracle -> state -> prog T -> @Result state T -> Prop :=
+
+  Inductive exec': forall T, oracle' -> state' -> prog' T -> @Result state' T -> Prop :=
   | ExecP1:
-      forall T (p1: O1.prog T) o1 s s1 r,
-        O1.exec o1 (fst s) p1 (Finished s1 r) ->
+      forall T (p1: L1.(prog) T) o1 s s1 r,
+        L1.(exec) o1 (fst s) p1 (Finished s1 r) ->
         exec' [Oracle1 o1] s (P1 p1) (Finished (s1, snd s) r)
-| ExecP2:
-      forall T (p2: O2.prog T) o2 s s2 r,
-        O2.exec o2 (snd s) p2 (Finished s2 r) ->
+  | ExecP2:
+      forall T (p2: L2.(prog) T) o2 s s2 r,
+        L2.(exec) o2 (snd s) p2 (Finished s2 r) ->
         exec' [Oracle2 o2] s (P2 p2) (Finished (fst s, s2) r)
-| ExecP1Crash:
-      forall T (p1: O1.prog T) o1 s s1,
-        O1.exec o1 (fst s) p1 (Crashed s1) ->
+  | ExecP1Crash:
+      forall T (p1: L1.(prog) T) o1 s s1,
+        L1.(exec) o1 (fst s) p1 (Crashed s1) ->
         exec' [Oracle1 o1] s (P1 p1) (Crashed (s1, snd s))
-| ExecP2Crash:
-      forall T (p2: O2.prog T) o2 s s2,
-        O2.exec o2 (snd s) p2 (Crashed s2) ->
+  | ExecP2Crash:
+      forall T (p2: L2.(prog) T) o2 s s2,
+        L2.(exec) o2 (snd s) p2 (Crashed s2) ->
         exec' [Oracle2 o2] s (P2 p2) (Crashed (fst s, s2)).
-  Definition exec := exec'.
-  Definition oracle_ok T (p: prog T) o s := 
+  
+  Definition weakest_precondition' T (p: prog' T) :=
     match p with
     | P1 p1 =>
+      fun Q o s =>
       exists o1,
-      o = [Oracle1 o1] /\ O1.oracle_ok p1 o1 (fst s)
+      o = [Oracle1 o1] /\ L1.(weakest_precondition) p1 (fun r s' => Q r (s', snd s)) o1 (fst s)
     | P2 p2 =>
+      fun Q o s =>
       exists o2,
-      o = [Oracle2 o2] /\ O2.oracle_ok p2 o2 (snd s)
+      o = [Oracle2 o2] /\ L2.(weakest_precondition) p2 (fun r s' => Q r (fst s, s')) o2 (snd s)
     end.
+
+  Definition weakest_crash_precondition' T (p: prog' T) :=
+    match p with
+    | P1 p1 =>
+      fun Q o s =>
+      exists o1,
+      o = [Oracle1 o1] /\ L1.(weakest_crash_precondition) p1 (fun s' => Q (s', snd s)) o1 (fst s)
+    | P2 p2 =>
+      fun Q o s =>
+      exists o2,
+      o = [Oracle2 o2] /\ L2.(weakest_crash_precondition) p2 (fun s' => Q (fst s, s')) o2 (snd s)
+    end.
+
+   Theorem wp_complete':
+      forall T (p: prog' T) H Q,
+        (forall o s, H o s -> weakest_precondition' p Q o s) <->
+        (forall o s, H o s ->
+                (exists s' v, exec' o s p (Finished s' v) /\ Q v s')).
+   Proof.
+     intros; destruct p; simpl.
+     {(* L1 *)
+       split; intros.
+       - specialize H0 with (1:= X); cleanup.
+         eapply wp_to_exec in H1; cleanup.
+         do 2 eexists; split; eauto.
+         econstructor; eauto.
+       - specialize H0 with (1:= X); cleanup.
+         inversion H0; cleanup.
+         eexists; split; eauto.
+         eapply exec_to_wp; eauto.
+     }
+     {(* L2 *)
+       split; intros.
+       - specialize H0 with (1:= X); cleanup.
+         eapply wp_to_exec in H1; cleanup.
+         do 2 eexists; split; eauto.
+         econstructor; eauto.
+       - specialize H0 with (1:= X); cleanup.
+         inversion H0; cleanup.
+         eexists; split; eauto.
+         eapply exec_to_wp; eauto.
+     }
+   Qed.
+       
+     
+   Theorem wcp_complete':
+     forall T (p: prog' T) H C,
+       (forall o s, H o s -> weakest_crash_precondition' p C o s) <->
+       (forall o s, H o s ->
+               (exists s', exec' o s p (Crashed s') /\ C s')).
+   Proof.
+     intros; destruct p; simpl.
+     {(* L1 *)
+       split; intros.
+       - specialize H0 with (1:= X); cleanup.
+         eapply wcp_to_exec in H1; cleanup.
+         eexists; split; eauto.
+         econstructor; eauto.
+       - specialize H0 with (1:= X); cleanup.
+         inversion H0; cleanup.
+         eexists; split; eauto.
+         eapply exec_to_wcp; eauto.
+     }
+     {(* L2 *)
+       split; intros.
+       - specialize H0 with (1:= X); cleanup.
+         eapply wcp_to_exec in H1; cleanup.
+         eexists; split; eauto.
+         econstructor; eauto.
+       - specialize H0 with (1:= X); cleanup.
+         inversion H0; cleanup.
+         eexists; split; eauto.
+         eapply exec_to_wcp; eauto.
+     }
+   Qed.
+   
   
-  Definition exec_deterministic_wrt_oracle :
-    forall o s T (p: prog T) ret1 ret2,
-      exec o s p ret1 ->
-      exec o s p ret2 ->
+  Definition exec_deterministic_wrt_oracle' :
+    forall o s T (p: prog' T) ret1 ret2,
+      exec' o s p ret1 ->
+      exec' o s p ret2 ->
       ret1 = ret2.
     intros; destruct p; simpl in *;
     inversion H; inversion H0;
     sigT_eq; clear H H0; cleanup;
-    try solve [eapply O1.exec_deterministic_wrt_oracle in H6;
-               eauto; cleanup; eauto];
-    try solve [eapply O2.exec_deterministic_wrt_oracle in H6;
+    try solve [eapply exec_deterministic_wrt_oracle in H6;
                eauto; cleanup; eauto].
-  Qed.
-    
-  Definition exec_then_oracle_ok:
-    forall T (p: prog T) o s r,
-      exec o s p r ->
-      oracle_ok p o s.
-    intros; destruct p; simpl in *;
-    inversion H; inversion H0;
-    sigT_eq; clear H H0; cleanup;
-    try solve [eapply O1.exec_then_oracle_ok in H5; eauto];
-    try solve [eapply O2.exec_then_oracle_ok in H5; eauto].
   Qed.
 
   Hint Constructors exec': core.
-  Hint Extern 0 (exec _ _ _ _ ) => econstructor : core.
-  
+
+  Definition HorizontalComposition :=
+    Build_Operation
+      oracle_dec' prog' exec'
+      weakest_precondition'
+      weakest_crash_precondition'
+      wp_complete' wcp_complete'
+      exec_deterministic_wrt_oracle'.
+
 End HorizontalComposition.
 
+Arguments P1 {O1 O2 L1 L2 T}.
+Arguments P2 {O1 O2 L1 L2 T}.
