src/Framework/Layer/Language.v
@@ -1,172 +1,120 @@
-Require Import Primitives Simulation.
+Require Import Primitives Layer.Operation.
 Import ListNotations.
 
 Set Implicit Arguments.
 
-Module Type Operation.
-  Parameter oracle : Type.
-  Parameter oracle_dec: forall (o o': oracle), {o = o'}+{o <> o'}.
-  Parameter state : Type.
-  Parameter prog : Type -> Type.
-  Parameter exec: forall T, oracle -> state -> prog T -> @Result state T -> Prop.
-  Parameter oracle_ok : forall T, prog T -> oracle -> state -> Prop.
-  Parameter exec_deterministic_wrt_oracle :
-    forall o s T (p: prog T) ret1 ret2,
-      exec o s p ret1 ->
-      exec o s p ret2 ->
-      ret1 = ret2.
-  Parameter exec_then_oracle_ok:
-    forall T (p: prog T) o s r,
-      exec o s p r ->
-      oracle_ok p o s.
-End Operation.
-
-Module Language (Op: Operation) <: Operation.
-  Import Op.
+Section Language.
   
-  Inductive token :=
-  | OpOracle : Op.oracle -> token
-  | Crash : token
-  | Cont : token.
+  Variable O: Operation.
 
-  Definition token_dec : forall (t t': token), {t=t'}+{t<>t'}.
+  Inductive token' :=
+  | OpOracle : O.(oracle) -> token'
+  | Crash : token'
+  | Cont : token'.
+
+  Definition token_dec' : forall (t t': token'), {t=t'}+{t<>t'}.
     decide equality.
-    apply oracle_dec.
+    apply O.(oracle_dec).
   Defined.
 
-  Definition oracle := list token.
-  Definition oracle_dec : forall (o o': oracle), {o=o'}+{o<>o'}.
+  Definition oracle' := list token'.
+  Definition oracle_dec' : forall (o o': oracle'), {o=o'}+{o<>o'}.
     repeat decide equality.
-    apply oracle_dec.
+    apply O.(oracle_dec).
   Defined.
 
 
-  Definition state := Op.state.
+  Definition state' := O.(state).
   
   Inductive prog' : Type -> Type :=
-  | Op : forall T, Op.prog T -> prog' T
+  | Op : forall T, O.(prog) T -> prog' T
   | Ret : forall T, T -> prog' T
   | Bind : forall T T', prog' T -> (T -> prog' T') -> prog' T'.
-
-  Definition prog := prog'.
   
   Inductive exec' :
-    forall T, oracle ->  state -> prog T -> @Result state T -> Prop :=
+    forall T, oracle' ->  state' -> prog' T -> @Result state' T -> Prop :=
   | ExecOp : 
-      forall T (p : Op.prog T) o s s' r,
-        Op.exec o s p (Finished s' r) ->
-        exec' [OpOracle o] s (Op p) (Finished s' r)
+      forall T (p : O.(prog) T) o s s' r,
+        O.(exec) o s p (Finished s' r) ->
+        exec' [OpOracle o] s (Op T p) (Finished s' r)
              
   | ExecRet :
       forall d T (v: T),
         exec' [Cont] d (Ret v) (Finished d v)
 
   | ExecBind :
-      forall T T' (p1: prog T) (p2: T -> prog T')
+      forall T T' (p1: prog' T) (p2: T -> prog' T')
         o1 d1 d1' o2 r ret,
         exec' o1 d1 p1 (Finished d1' r) ->
         exec' o2 d1' (p2 r) ret ->
         exec' (o1++o2) d1 (Bind p1 p2) ret
 
   | ExecOpCrash : 
-      forall T (p : Op.prog T) o s s',
-        Op.exec o s p (Crashed s') ->
-        exec' [OpOracle o] s (Op p) (Crashed s')
+      forall T (p : O.(prog) T) o s s',
+        O.(exec) o s p (Crashed s') ->
+        exec' [OpOracle o] s (Op T p) (Crashed s')
              
   | ExecRetCrash :
       forall T d (v: T),
         exec' [Crash] d (Ret v) (Crashed d)
              
   | ExecBindCrash :
-      forall T T' (p1: prog T) (p2: T -> prog T')
+      forall T T' (p1: prog' T) (p2: T -> prog' T')
         o1 o2 d1 d1',
         exec' o1 d1 p1 (Crashed d1') ->
         exec' (o1++o2) d1 (Bind p1 p2) (Crashed d1').
 
-  Definition exec := exec'.
-  
-  Fixpoint oracle_ok {T} (p: prog T) o s :=
-    match p with
+  Fixpoint weakest_precondition' T (p: prog' T) :=    
+      match p with
     | Bind p1 p2 =>
-      exists o1 o2,
+      fun Q o s =>
+        exists o1 o2,
       o = o1++o2 /\
-      oracle_ok p1 o1 s /\
-      (forall s' r,
-          exec o1 s p1 (Finished s' r) ->
-          oracle_ok (p2 r) o2 s') 
-    | Op p' =>
-      exists o',
+      weakest_precondition' p1 (fun r s' => weakest_precondition' (p2 r) Q o2 s') o1 s
+    | Op T' p' =>
+      fun Q o s =>
+        exists o',
       o = [OpOracle o'] /\
-      Op.oracle_ok p' o' s
-    | Ret _ =>
-      o = [Cont] \/ o = [Crash]
+      O.(weakest_precondition) p' Q o' s
+    | Ret v =>
+      fun Q o s =>
+        o = [Cont] /\ Q v s
+      end.
+
+  Fixpoint weakest_crash_precondition' T (p: prog' T) :=    
+      match p with
+    | Bind p1 p2 =>
+      fun Q (o: oracle') s =>
+        exists o1 o2,
+          o = o1++o2 /\
+          (weakest_crash_precondition' p1 Q o1 s \/
+           (exists s' r,
+              exec' o1 s p1 (Finished s' r) /\
+              weakest_crash_precondition' (p2 r) Q o2 s'))
+    | Op T' p' =>
+      fun Q o s =>
+        exists o',
+      o = [OpOracle o'] /\
+      O.(weakest_crash_precondition) p' Q o' s
+    | Ret v =>
+      fun Q o s =>
+        o = [Crash] /\ Q s
     end.
 
-  Definition lts := Build_LTS oracle state prog exec.
-  
-  Notation "| p |" := (Op p)(at level 60).
-  Notation "x <- p1 ; p2" := (Bind p1 (fun x => p2))(right associativity, at level 60).
-  Notation "x <-| p1 ; p2" := (Bind (Op p1) (fun x => p2))(right associativity, at level 60).
-  Hint Constructors exec'.
-  Hint Extern 0 (exec _ _ (Op _) _ ) => econstructor.
-  Hint Extern 0 (exec _ _ _ _ ) => econstructor.
+  Hint Constructors exec' : core.
+
   (* Automation *)
-  Local Ltac invert_exec'' H :=
-  inversion H; subst; clear H; repeat sigT_eq.
+(*
 
-  Local Ltac invert_exec' :=
-  match goal with
-  | [ H: exec _ _ ?p _ |- _ ] =>
-    match p with
-    | Bind _ _ => idtac
-    | Op _ => invert_exec'' H
-    | Ret _ => invert_exec'' H
-    end
-  end.
-
-Lemma bind_sep:
-  forall T T' o d (p1: prog T) (p2: T -> prog T') ret,
-    exec o d (Bind p1 p2) ret ->
-    match ret with
-    | Finished d' r =>
-    (exists o1 o2 d1 r1,
-       exec o1 d p1 (Finished d1 r1) /\
-       exec o2 d1 (p2 r1) ret /\
-       o = o1++o2)
-  | Crashed d' =>
-    (exists o1 o2,
-    o = o1++o2 /\    
-    (exec o1 d p1 (Crashed d') \/
-     (exists d1 r1,
-        exec o1 d p1 (Finished d1 r1) /\
-        exec o2 d1 (p2 r1) ret)))
-    end.
-Proof.
-  intros.
-  invert_exec'' H; eauto.
-  destruct ret.
-  do 2 eexists; eauto.
-  do 2 eexists; split; eauto.
-Qed.
-
-Ltac invert_exec :=
-  match goal with
-  |[H : exec _ _ (Bind _ _) _ |- _ ] =>
-   apply bind_sep in H; repeat cleanup
-  |[H : exec _ _ _ _ |- _ ] =>
-   invert_exec'
-  end.
-
-
-  Definition prog_equiv T : prog T -> prog T -> Prop :=
+  Definition prog_equiv T : prog' T -> prog' T -> Prop :=
     fun p1 p2 => forall o d out,
-        exec o d p1 out <-> exec o d p2 out.
+        exec' o d p1 out <-> exec' o d p2 out.
 
   Arguments prog_equiv {T} _ _.
 
   Infix "~=" := prog_equiv (at level 50, left associativity).
 
-  Theorem bind_assoc : forall T T' T'' (p1: prog T) (p2: T -> prog T') (p3: T' -> prog T''),
+  Theorem bind_assoc : forall T T' T'' (p1: prog' T) (p2: T -> prog' T') (p3: T' -> prog' T''),
       Bind (Bind p1 p2) p3 ~= Bind p1 (fun x => Bind (p2 x) p3).
   Proof.
     split; intros.
@@ -203,128 +151,28 @@ Ltac invert_exec :=
       rewrite app_assoc.
       repeat econstructor; eauto.
   Qed.
-
-  (* Facts *)
-
-  (*
-Lemma exec_crash_in:
-  forall T (p: prog T) o d d',
-    exec o d p (Crashed d') ->
-    In Crash o.
-Proof.
-  induction p; simpl in *; intros;
-    try invert_exec; intuition; eauto.
-  cleanup.
-  apply in_app_iff; eauto.
-Qed.
 *)
-
-Lemma exec_finished_deterministic_prefix:
-  forall T (p: prog T) o1 o2 o3 o4 s s1 s2 r1 r2,
-      exec o1 s p (Finished s1 r1) ->
-      exec o2 s p (Finished s2 r2) ->
-      o1 ++ o3 = o2 ++ o4 ->
-      o1 = o2 /\ s1 = s2 /\ r1 = r2.
+    
+(*  
+Lemma exec_crashed_oracle_app:
+  forall T (p: prog T) o1 o2 s s1,
+    exec o1 s p (Crashed s1) ->
+    exec (o1++o2) s p (Crashed s1).
 Proof.
   induction p; simpl; intros;
-    repeat (invert_exec; simpl in *; cleanup);
-    simpl; eauto; try solve [intuition].
-  eapply Op.exec_deterministic_wrt_oracle in H7; eauto; cleanup; eauto.
-  
-  repeat rewrite <- app_assoc in H2.
-  specialize IHp with (1:= H0)(2:= H1)(3:=H2); cleanup.
-  specialize H with (1:= H4)(2:= H3)(3:=H2); cleanup; eauto.
-Qed.
-
-Lemma finished_not_crashed_oracle_prefix:
-  forall T (p: prog T) o1 o2 o3 o4 s s1 s2 r1,
-    exec o1 s p (Finished s1 r1) ->
-    o1 ++ o3 = o2 ++ o4 ->
-    ~exec o2 s p (Crashed s2).
-Proof.
-  unfold not; induction p; simpl; intros;
-    repeat (invert_exec; simpl in *; cleanup); simpl; eauto.
-  eapply exec_deterministic_wrt_oracle in H7; eauto; cleanup.
+  repeat (invert_exec; simpl in *; cleanup); simpl; eauto.
   
   split_ors; cleanup.
   -
-    repeat rewrite <- app_assoc in H1; eauto.
+    rewrite <- app_assoc; eapply ExecBindCrash; eauto.
+
   -
-    repeat rewrite <- app_assoc in H1; eauto.
-    eapply exec_finished_deterministic_prefix in H0; eauto; cleanup; eauto.
+    rewrite <- app_assoc; econstructor; eauto.
+    eapply H in H1; eauto.
 Qed.
-
-Lemma finished_not_crashed_oracle_app:
-  forall T (p: prog T) o1 o2 s s1 s2 r1,
-    exec o1 s p (Finished s1 r1) ->
-    ~exec (o1++o2) s p (Crashed s2).
-Proof.
-  unfold not; induction p; simpl; intros;
-    repeat (invert_exec; simpl in *; cleanup); simpl; eauto.
-  eapply exec_deterministic_wrt_oracle in H6; eauto; cleanup.
-  
-  split_ors; cleanup.
-  -
-    rewrite <- app_assoc in H1; eauto.
-    clear H3; eapply finished_not_crashed_oracle_prefix; eauto.
-  -
-    rewrite <- app_assoc in H1; eauto.
-    eapply exec_finished_deterministic_prefix in H0; eauto; cleanup; eauto.
-Qed.
-
-Lemma exec_deterministic_wrt_oracle_prefix:
-      forall T (p: prog T) o1 o2 x1 x2 s ret1 ret2,
-      exec o1 s p ret1 -> 
-      exec x1 s p ret2 ->
-      o1 ++ o2 = x1 ++ x2 ->
-      ret1 = ret2.
-    Proof.
-       induction p; simpl; intros;
-    repeat (invert_exec; simpl in *; cleanup);
-    simpl; eauto; try solve [intuition].
-  -
-    eapply Op.exec_deterministic_wrt_oracle; eauto.
-  -
-    eapply Op.exec_deterministic_wrt_oracle in H6; eauto; cleanup.
-  -
-    eapply Op.exec_deterministic_wrt_oracle in H6; eauto; cleanup.
-  -
-    eapply Op.exec_deterministic_wrt_oracle; eauto; cleanup.
-  -
-    eapply exec_finished_deterministic_prefix in H0; eauto; cleanup; eauto.
-    repeat rewrite <- app_assoc in H2; cleanup; eauto.
-    repeat rewrite <- app_assoc in H2; eauto.
-  -
-    split_ors; cleanup.
-    repeat rewrite <- app_assoc in H2; eauto.
-    specialize IHp with (1:=H0)(2:=H1)(3:=H2); cleanup.
-
-    repeat rewrite <- app_assoc in H2.
-    eapply exec_finished_deterministic_prefix in H0; eauto; cleanup; eauto.
+ *)
     
-  -
-    split_ors; cleanup.
-    repeat rewrite <- app_assoc in H2; eauto.
-    specialize IHp with (1:=H0)(2:=H3)(3:=H2); cleanup.
-
-    repeat rewrite <- app_assoc in H2.
-    eapply exec_finished_deterministic_prefix in H0; eauto; cleanup; eauto.
-  -
-    repeat split_ors; cleanup.
-    repeat rewrite <- app_assoc in H2; eauto.
-    specialize IHp with (1:= H1)(2:= H0)(3:=H2); cleanup; eauto.
-
-    repeat rewrite <- app_assoc in H2; eauto.
-    specialize IHp with (1:=H1)(2:=H0)(3:=H2); cleanup.
-
-    repeat rewrite <- app_assoc in H2; eauto.
-    specialize IHp with (1:=H1)(2:=H0)(3:=H2); cleanup.
-
-    repeat rewrite <- app_assoc in H2.
-    eapply exec_finished_deterministic_prefix in H1; eauto; cleanup; eauto.
-    Qed.
-
-    (*
+(*
 Lemma oracle_nonempty_app_not_crashed:
   forall T (p: prog T) o1 o2 s s1 ret,
     exec o1 s p ret ->
@@ -377,76 +225,6 @@ Qed.
 
 *)
 
-Lemma exec_deterministic_wrt_oracle:
-  forall o s T (p: prog T) r1 r2,
-      exec o s p r1 ->
-      exec o s p r2 ->
-      r1 = r2.
-Proof.
-  intros.
-  eapply exec_deterministic_wrt_oracle_prefix; eauto.
-  Unshelve.
-  eauto.
-Qed.
-
-  Lemma oracle_ok_nonempty:
-    forall T (p: prog T) s,
-      ~oracle_ok p [] s.
-  Proof.
-    unfold not;
-      induction p; simpl; intros; try (split_ors; cleanup); try intuition congruence.
-    cleanup; inversion H. 
-    cleanup; symmetry in H0; apply app_eq_nil in H0; cleanup; eauto.
-  Qed.
-
-  Lemma oracle_ok_bind_assoc:
-    forall T T' T'' (p1: prog T) (p2: T -> prog T') (p3: T' -> prog T'') o sl,
-      oracle_ok (Bind (Bind p1 p2) p3) o sl ->
-      oracle_ok (Bind p1 (fun x => (Bind (p2 x) p3))) o sl.      
-  Proof.
-    intros; simpl in *; cleanup.
-    exists x1, (x2++x0).
-    split.
-    rewrite app_assoc; eauto.
-    intuition eauto.
-    specialize H3 with (1:= H).
-    do 2 eexists; intuition eauto.
-  Qed.
-  
-  Lemma oracle_ok_bind_finished_split:
-    forall T T' (p1: prog T) (p2: T -> prog T') o1 o2 sl sl' r ret,
-      exec o1 sl p1 (Finished sl' r) ->
-      exec o2 sl' (p2 r) ret ->
-      oracle_ok (Bind p1 p2) (o1 ++ o2) sl ->
-      oracle_ok p1 o1 sl /\
-      oracle_ok (p2 r) o2 sl'.      
-  Proof.
-    induction p1; simpl; intros;
-    try solve [  pose proof H;
-      simpl in *; intuition;
-        invert_exec; simpl in *; cleanup;
-      split_ors; cleanup; inversion H1; subst; eauto;
-      specialize H3 with (1:= H); eauto].
-    invert_exec; simpl in *; cleanup; simpl in *; split;
-      inversion H; subst; eauto.
-    
-    invert_exec.
-    repeat rewrite <- app_assoc in H2.
-    specialize (IHp1 (fun x => Bind (p x) p2)) with (1:=H0).
-    edestruct IHp1.
-    econstructor; eauto.
-    rewrite H2.
-    econstructor; eexists; intuition eauto.
-    specialize H6 with (1:=H3).
-    econstructor; eexists; intuition eauto.
-
-    specialize H with (1:=H7)(2:= H1).
-    destruct H; intuition eauto.
-    
-    simpl in *; cleanup.
-    do 2 eexists; intuition eauto.
-    eapply exec_deterministic_wrt_oracle in H0; eauto; cleanup; eauto.
-  Qed.
 (*
   Lemma oracle_ok_finished_eq:
     forall T (p: prog T) o1 o2 o1' o2' s s' r,
@@ -489,43 +267,45 @@ Qed.
        specialize H3 with (1:=H0).
        specialize H with (1:= H1)(2:=H3); eauto.
   Qed.
+ *)
 
-   Lemma oracle_ok_bind_crashed_split:
-    forall T T' (p1: prog T) (p2: T -> prog T') o1 sl sl',
-      exec o1 sl p1 (Crashed sl') ->
-      oracle_ok (Bind p1 p2) o1 sl ->
-      oracle_ok p1 o1 sl.      
+
+(*
+    Lemma oracle_ok_bind_finished_split:
+    forall T T' (p1: prog T) (p2: T -> prog T') o1 o2 sl sl' r ret,
+      exec o1 sl p1 (Finished sl' r) ->
+      exec o2 sl' (p2 r) ret ->
+      oracle_ok (Bind p1 p2) (o1 ++ o2) sl ->
+      oracle_ok p1 o1 sl /\
+      oracle_ok (p2 r) o2 sl'.      
   Proof.
-    intros; simpl in *; cleanup.
-    eapply_fresh oracle_ok_exec_crashed_app_nil in H; eauto; cleanup.
-    rewrite app_nil_r; eauto.
-  Qed.
-*)
-   Lemma exec_then_oracle_ok:
-    forall T (p: prog T) o s r,
-      exec o s p r ->
-      oracle_ok p o s.
-  Proof.
-    induction p; simpl; intros; try solve [invert_exec; cleanup; simpl; eauto].
-    invert_exec; cleanup; simpl; eauto; eapply exec_then_oracle_ok in H5; eauto.
+    induction p1; simpl; intros;
+    try solve [  pose proof H;
+      simpl in *; intuition;
+        invert_exec; simpl in *; cleanup;
+      split_ors; cleanup; inversion H1; subst; eauto;
+      specialize H3 with (1:= H); eauto].    
+    invert_exec; simpl in *; cleanup; simpl in *; split;
+      inversion H; subst; eauto.
     
     invert_exec.
-    - specialize IHp with (1:= H0).
-      specialize H with (1:=H1).
-      do 2 eexists; intuition; eauto;
-        eapply exec_deterministic_wrt_oracle in H0; eauto; cleanup; eauto.
-    -
-      split_ors; cleanup.
-      specialize IHp with (1:= H0).
-      do 2 eexists; intuition; eauto;
-        eapply exec_deterministic_wrt_oracle in H0; eauto; cleanup; eauto.
+    repeat rewrite <- app_assoc in H2.
+    specialize (IHp1 (fun x => Bind (p x) p2)) with (1:=H0).
+    edestruct IHp1.
+    econstructor; eauto.
+    rewrite H2.
+    econstructor; eexists; intuition eauto.
+    specialize H6 with (1:=H3).
+    econstructor; eexists; intuition eauto.
 
-      specialize IHp with (1:= H0).
-      specialize H with (1:=H1).
-      do 2 eexists; intuition; eauto;
-        eapply exec_deterministic_wrt_oracle in H0; eauto; cleanup; eauto.
+    specialize H with (1:=H7)(2:= H1).
+    destruct H; intuition eauto.
+    
+    simpl in *; cleanup.
+    do 2 eexists; intuition eauto.
+    eapply exec_deterministic_wrt_oracle in H0; eauto; cleanup; eauto.
   Qed.
-
+*)
   (*
   Lemma finished_crash_not_in:
     forall T (p: prog T) s s' o r,
@@ -535,8 +315,337 @@ Qed.
     induction p; simpl; intros; invert_exec; cleanup; simpl; intuition eauto; try congruence.
     apply in_app_iff in H2; intuition eauto.
   Qed.
-  *)
-
+   *)
+Record Language :=
+  {
+    token := token';
+    token_dec := token_dec';
+    oracle := oracle';
+    oracle_dec := oracle_dec';
+    state := state';
+    prog := prog';
+    exec := exec';
+    weakest_precondition := weakest_precondition';
+    weakest_crash_precondition := weakest_crash_precondition'
+  }.
 
 End Language.
 
+Arguments Ret {O T}.
+Hint Extern 1 (Language.exec _ _ _ (Op _ _ _) (Finished _ _)) => eapply (ExecOp _) : core.
+Notation "| p |" := (Language.Op _ _ p)(at level 60).
+Notation "x <- p1 ; p2" := (Bind p1 (fun x => p2))(right associativity, at level 60).
+Notation "x <-| p1 ; p2" := (Bind (Op _ _ p1) (fun x => p2))(right associativity, at level 60).
+
+  Local Ltac invert_exec'' H :=
+  inversion H; subst; clear H; repeat sigT_eq.
+
+  Local Ltac invert_exec' :=
+  match goal with
+  | [ H: exec _ _ _ ?p _ |- _ ] =>
+    match p with
+    | Bind _ _ => idtac
+    | Op _ _ _ => invert_exec'' H
+    | Ret _ => invert_exec'' H
+    end
+  end.
+
+Lemma bind_sep:
+  forall O (L: Language O) T T' o d (p1: prog L T) (p2: T -> prog L T') ret,
+    exec L o d (Bind p1 p2) ret ->
+    match ret with
+    | Finished d' r =>
+    (exists o1 o2 d1 r1,
+       exec L o1 d p1 (Finished d1 r1) /\
+       exec L o2 d1 (p2 r1) ret /\
+       o = o1++o2)
+  | Crashed d' =>
+    (exists o1 o2,
+    o = o1++o2 /\    
+    (exec L o1 d p1 (Crashed d') \/
+     (exists d1 r1,
+        exec L o1 d p1 (Finished d1 r1) /\
+        exec L o2 d1 (p2 r1) ret)))
+    end.
+Proof.
+  intros.
+  invert_exec'' H; eauto.
+  destruct ret.
+  do 2 eexists; eauto.
+  do 2 eexists; split; eauto.
+Qed.
+
+Ltac invert_exec :=
+  match goal with
+  |[H : exec _ _ _ (Bind _ _) _ |- _ ] =>
+   apply bind_sep in H; repeat cleanup
+  |[H : exec _ _ _ _ _ |- _ ] =>
+   invert_exec'
+  end.
+
+Lemma wp_complete :
+  forall O (L: Language O) T (p: L.(prog) T) H Q,
+        (forall o s, H o s -> L.(weakest_precondition) p Q o s) <->
+        (forall o s, H o s ->
+                (exists s' v, L.(exec) o s p (Finished s' v) /\ Q v s')).
+Proof.
+  induction p; intros.
+  { (* Op *)
+    simpl; split; intros.
+    - specialize H0 with (1:=X); cleanup.
+      eapply wp_to_exec in H1; eauto; cleanup; eauto.
+      
+    - specialize H0 with (1:=X); cleanup.
+      invert_exec.
+      eapply exec_to_wp in H1; eauto.
+  }
+  {(* Ret *)
+    simpl; split; intros.
+    - specialize H0 with (1:=X); cleanup; eauto.
+      do 2 eexists; intuition eauto.
+      econstructor; eauto.
+      
+    - specialize H0 with (1:=X); cleanup.
+      invert_exec; eauto.
+  }
+  {(*Bind*)
+    simpl in *; split; intros.
+    - specialize H1 with (1:=X); cleanup; eauto.
+      edestruct IHp.
+      edestruct H1; eauto; simpl in *; cleanup.
+      edestruct H.
+      edestruct H6; eauto; simpl in *; cleanup.      
+      do 2 eexists; intuition eauto.
+      econstructor; eauto.
+
+    - specialize H1 with (1:=X); cleanup.
+      invert_exec; eauto.
+      do 2 eexists; intuition eauto.
+      eapply IHp.
+      intros.
+      do 2 eexists; intuition eauto.
+      instantiate (1:= fun o s => exec L o s p (Finished x3 x4)) in X0; simpl in *; eauto.
+            
+      eapply H; intros; eauto.  
+      do 2 eexists; intuition eauto.
+      instantiate (1:= fun o s => exec L o s (p0 x4) (Finished x x0)) in X1; simpl in *; eauto.
+      all: simpl in *; eauto.
+  }
+Qed.
+
+Lemma wcp_complete :
+  forall O (L: Language O) T (p: L.(prog) T) H Q,
+        (forall o s, H o s -> L.(weakest_crash_precondition) p Q o s) <->
+        (forall o s, H o s ->
+                (exists s', L.(exec) o s p (Crashed s') /\ Q s')).
+Proof.
+  induction p; intros.
+  { (* Op *)
+    simpl; split; intros.
+    - specialize H0 with (1:=X); cleanup.
+      eapply wcp_to_exec in H1; eauto; cleanup; eauto.
+      do 2 eexists; eauto.
+      eapply ExecOpCrash; eauto.
+      
+    - specialize H0 with (1:=X); cleanup.
+      invert_exec.
+      eapply exec_to_wcp in H1; eauto.
+  }
+  {(* Ret *)
+    simpl; split; intros.
+    - specialize H0 with (1:=X); cleanup; eauto.
+      do 2 eexists; intuition eauto.
+      econstructor; eauto.
+      
+    - specialize H0 with (1:=X); cleanup.
+      invert_exec; eauto.
+  }
+  {(*Bind*)
+    simpl in *; split; intros.
+    - specialize H1 with (1:=X); cleanup; eauto.
+      split_ors.
+      + edestruct IHp.
+        edestruct H2; eauto; simpl in *; cleanup.
+        eexists. intuition eauto. eapply ExecBindCrash; eauto.
+      + edestruct H.
+        eapply H3 in H2; eauto; simpl in *; cleanup.      
+        eexists; intuition eauto.
+        econstructor; eauto.
+
+    - specialize H1 with (1:=X); cleanup.
+      invert_exec; eauto.
+      split_ors.
+      + do 2 eexists; intuition eauto.
+        left; eapply IHp.
+        intros.
+        eexists; intuition eauto.
+        instantiate (1:= fun o s => exec L o s p (Crashed x)) in X0; simpl in *; eauto.
+        simpl; eauto.
+            
+      + do 2 eexists; intuition eauto.
+        right; do 2 eexists; split; eauto.
+        eapply H.
+        intros.
+        eexists; intuition eauto.
+        instantiate (1:= fun o s => exec L o s (p0 x3) (Crashed x)) in X0; simpl in *; eauto.
+        simpl; eauto.
+  }
+Qed.
+
+
+Lemma wp_to_exec:
+  forall O (L: Language O) T (p: prog L T) Q o s,
+    weakest_precondition L p Q o s -> (exists s' v, exec L o s p (Finished s' v) /\ Q v s').
+Proof.
+  intros. eapply wp_complete; eauto.
+Qed.
+
+Lemma exec_to_wp:
+  forall O (L: Language O) T (p: prog L T) (Q: T -> state L -> Prop) o s s' v,
+    exec L o s p (Finished s' v) ->
+    Q v s' ->
+    weakest_precondition L p Q o s.
+Proof.
+  intros.
+  eapply wp_complete; intros.
+  apply X.
+  simpl; eauto.
+Qed.
+
+Lemma wcp_to_exec:
+  forall O (L: Language O) T (p: L.(prog) T) Q o s,
+    weakest_crash_precondition L p Q o s -> (exists s', exec L o s p (Crashed s') /\ Q s').
+Proof.
+  intros. eapply wcp_complete; eauto.
+Qed.
+  
+Lemma exec_to_wcp:
+  forall O (L: Language O) T (p: L.(prog) T) (Q: state L -> Prop) o s s',
+    exec L o s p (Crashed s') ->
+    Q s' ->
+    weakest_crash_precondition L p Q o s.
+Proof.
+  intros.
+  eapply wcp_complete; intros.
+  apply X.
+  simpl; eauto.
+Qed.
+
+  (* Facts *)
+
+Lemma exec_finished_deterministic_prefix:
+  forall O (L: Language O) T (p: prog L T) o1 o2 o3 o4 s s1 s2 r1 r2,
+      exec L o1 s p (Finished s1 r1) ->
+      exec L o2 s p (Finished s2 r2) ->
+      o1 ++ o3 = o2 ++ o4 ->
+      o1 = o2 /\ s1 = s2 /\ r1 = r2.
+Proof.
+  induction p; simpl; intros;
+    repeat (invert_exec; simpl in *; cleanup);
+    simpl; eauto; try solve [intuition].
+  eapply O.(exec_deterministic_wrt_oracle) in H7; eauto; cleanup; eauto.
+  
+  repeat rewrite <- app_assoc in H2.
+  specialize IHp with (1:= H0)(2:= H1)(3:=H2); cleanup.
+  specialize H with (1:= H4)(2:= H3)(3:=H2); cleanup; eauto.
+Qed.
+
+Lemma finished_not_crashed_oracle_prefix:
+  forall O (L: Language O) T (p: prog L T) o1 o2 o3 o4 s s1 s2 r1,
+    exec L o1 s p (Finished s1 r1) ->
+    o1 ++ o3 = o2 ++ o4 ->
+    ~exec L o2 s p (Crashed s2).
+Proof.
+  unfold not; induction p; simpl; intros;
+    repeat (invert_exec; simpl in *; cleanup); simpl; eauto.
+  eapply exec_deterministic_wrt_oracle in H7; eauto; cleanup.
+  
+  split_ors; cleanup.
+  -
+    repeat rewrite <- app_assoc in H1; eauto.
+  -
+    repeat rewrite <- app_assoc in H1; eauto.
+    eapply exec_finished_deterministic_prefix in H0; eauto; cleanup; eauto.
+Qed.
+
+Lemma finished_not_crashed_oracle_app:
+  forall O (L: Language O) T (p: prog L T) o1 o2 s s1 s2 r1,
+    exec L o1 s p (Finished s1 r1) ->
+    ~exec L (o1++o2) s p (Crashed s2).
+Proof.
+  unfold not; induction p; simpl; intros;
+    repeat (invert_exec; simpl in *; cleanup); simpl; eauto.
+  eapply exec_deterministic_wrt_oracle in H6; eauto; cleanup.
+  
+  split_ors; cleanup.
+  -
+    rewrite <- app_assoc in H1; eauto.
+    clear H3; eapply finished_not_crashed_oracle_prefix; eauto.
+  -
+    rewrite <- app_assoc in H1; eauto.
+    eapply exec_finished_deterministic_prefix in H0; eauto; cleanup; eauto.
+Qed.
+
+Lemma exec_deterministic_wrt_oracle_prefix:
+      forall O (L: Language O) T (p: prog L T) o1 o2 x1 x2 s ret1 ret2,
+      exec L o1 s p ret1 -> 
+      exec L x1 s p ret2 ->
+      o1 ++ o2 = x1 ++ x2 ->
+      ret1 = ret2.
+    Proof.
+       induction p; simpl; intros;
+    repeat (invert_exec; simpl in *; cleanup);
+    simpl; eauto; try solve [intuition].
+  -
+    eapply O.(exec_deterministic_wrt_oracle); eauto.
+  -
+    eapply O.(exec_deterministic_wrt_oracle) in H6; eauto; cleanup.
+  -
+    eapply O.(exec_deterministic_wrt_oracle) in H6; eauto; cleanup.
+  -
+    eapply O.(exec_deterministic_wrt_oracle); eauto; cleanup.
+  -
+    eapply exec_finished_deterministic_prefix in H0; eauto; cleanup; eauto.
+    repeat rewrite <- app_assoc in H2; cleanup; eauto.
+    repeat rewrite <- app_assoc in H2; eauto.
+  -
+    split_ors; cleanup.
+    repeat rewrite <- app_assoc in H2; eauto.
+    specialize IHp with (1:=H0)(2:=H1)(3:=H2); cleanup.
+
+    repeat rewrite <- app_assoc in H2.
+    eapply exec_finished_deterministic_prefix in H0; eauto; cleanup; eauto.
+    
+  -
+    split_ors; cleanup.
+    repeat rewrite <- app_assoc in H2; eauto.
+    specialize IHp with (1:=H0)(2:=H3)(3:=H2); cleanup.
+
+    repeat rewrite <- app_assoc in H2.
+    eapply exec_finished_deterministic_prefix in H0; eauto; cleanup; eauto.
+  -
+    repeat split_ors; cleanup.
+    repeat rewrite <- app_assoc in H2; eauto.
+    specialize IHp with (1:= H1)(2:= H0)(3:=H2); cleanup; eauto.
+
+    repeat rewrite <- app_assoc in H2; eauto.
+    specialize IHp with (1:=H1)(2:=H0)(3:=H2); cleanup.
+
+    repeat rewrite <- app_assoc in H2; eauto.
+    specialize IHp with (1:=H1)(2:=H0)(3:=H2); cleanup.
+
+    repeat rewrite <- app_assoc in H2.
+    eapply exec_finished_deterministic_prefix in H1; eauto; cleanup; eauto.
+ Qed.
+    
+Lemma exec_deterministic_wrt_oracle:
+  forall O (L: Language O) T (p: prog L T) o s r1 r2,
+      exec L o s p r1 ->
+      exec L o s p r2 ->
+      r1 = r2.
+Proof.
+  intros.
+  eapply exec_deterministic_wrt_oracle_prefix; eauto.
+  Unshelve.
+  eauto.
+Qed.
