src/Framework/Layer/Operation.v
@@ -1,0 +1,72 @@
+Require Import Primitives.
+Import ListNotations.
+
+Set Implicit Arguments.
+
+Record Operation :=
+  {
+    oracle : Type;
+    oracle_dec: forall (o o': oracle), {o = o'}+{o <> o'};
+    state : Type;
+    prog : Type -> Type;
+    exec: forall T, oracle -> state -> prog T -> @Result state T -> Prop;
+    weakest_precondition: forall T, prog T -> (T -> state -> Prop) -> (oracle -> state -> Prop);
+    weakest_crash_precondition: forall T, prog T -> (state -> Prop) -> (oracle -> state -> Prop);
+    wp_complete:
+      forall T (p: prog T) H Q,
+        (forall o s, H o s -> weakest_precondition p Q o s) <->
+        (forall o s, H o s ->
+                (exists s' v, exec o s p (Finished s' v) /\ Q v s'));
+    wcp_complete:
+      forall T (p: prog T) H C,
+        (forall o s, H o s -> weakest_crash_precondition p C o s) <->
+        (forall o s, H o s ->
+            (exists s', exec o s p (Crashed s') /\ C s'));
+      exec_deterministic_wrt_oracle :
+        forall o s T (p: prog T) ret1 ret2,
+          exec o s p ret1 ->
+          exec o s p ret2 ->
+          ret1 = ret2;
+  }.
+
+Arguments exec _ {T}.
+Arguments weakest_precondition _ {T}.
+Arguments weakest_crash_precondition _ {T}.
+
+Lemma wp_to_exec:
+  forall O T (p: @prog O T) Q o s,
+    weakest_precondition _ p Q o s -> (exists s' v, exec _ o s p (Finished s' v) /\ Q v s').
+Proof.
+  intros. eapply wp_complete; eauto.
+Qed.
+
+Lemma exec_to_wp:
+  forall O T (p: @prog O T) (Q: T -> state _ -> Prop) o s s' v,
+    exec _ o s p (Finished s' v) ->
+    Q v s' ->
+    weakest_precondition _ p Q o s.
+Proof.
+  intros.
+  eapply wp_complete; intros.
+  apply X.
+  simpl; eauto.
+Qed.
+
+Lemma wcp_to_exec:
+  forall O T (p: O.(@prog) T) Q o s,
+    weakest_crash_precondition _ p Q o s -> (exists s', exec _ o s p (Crashed s') /\ Q s').
+Proof.
+  intros. eapply wcp_complete; eauto.
+Qed.
+  
+Lemma exec_to_wcp:
+  forall O T (p: O.(@prog) T) (Q: state _ -> Prop) o s s',
+    exec _ o s p (Crashed s') ->
+    Q s' ->
+    weakest_crash_precondition _ p Q o s.
+Proof.
+  intros.
+  eapply wcp_complete; intros.
+  apply X.
+  simpl; eauto.
+Qed.
