src/Framework/Simulation/Simulation.v
@@ -1,1 +1,1 @@
-Require Export Simulation.Definitions Simulation.Metatheory.
+Require Export Simulation.Definitions Simulation.WeakestPreconditions Simulation.Metatheory.
